src/examples/Kuiper.Example.Mul.fst
@@ -11,28 +11,24 @@ let smul (s1 : seq u64) (s2 : seq u64 { len s2 == len s1 })
   = Seq.init (len s1) (fun i -> U64.mul_mod s1.[i] s2.[i])
 
 [@@CPrologue "__device__"] // no KrmlPrivate, example
-fn kf (#size : erased nat{size > 0}) (* do NOT use erased pos, inference suffers *)
-  (a1 a2 ar : gpu_array u64 size)
+fn kf (#size : erased nat)
+  (a1 a2 ar : larray u64 size)
   (s1 s2 : erased (seq u64))
   (#_ : squash (len s1 == size /\ len s2 == size))
   (bid : szlt size)
   preserves
-    gpu ** block_id size bid **
-    pts_to a1 #(1.0R /. size) s1 **
-    pts_to a2 #(1.0R /. size) s2 **
-    emp
+    pts_to_slice a1 #(1.0R /. size) 0 size s1 **
+    pts_to_slice a2 #(1.0R /. size) 0 size s2
   requires
-    gpu_pts_to_slice ar bid (bid + 1) 's
+    pts_to_slice ar bid (bid + 1) 's
   ensures
-    gpu_pts_to_slice ar bid (bid + 1) seq![(smul s1 s2).[bid]]
+    pts_to_slice ar bid (bid + 1) seq![(smul s1 s2).[bid]]
 {
-  assert (pure (bid >= 0));
-  assert (pure (bid < size));
-  let v1 = gpu_array_read a1 bid;
-  let v2 = gpu_array_read a2 bid;
+  let v1 = slice_read a1 bid;
+  let v2 = slice_read a2 bid;
   let v = FStar.UInt64.(v1 *%^ v2);
-  gpu_array_write ar bid v;
-  (**)with sr. assert gpu_pts_to_slice ar bid (bid + 1) sr;
+  slice_write ar bid v;
+  (**)with sr. assert pts_to_slice ar bid (bid + 1) sr;
   (**)Seq.lemma_eq_intro sr seq![(smul s1 s2).[bid]];
   ()
 }
