src/lib/kuiper/Kuiper.Array.Derived.fst
@@ -21,31 +21,34 @@ open Kuiper.Array.Core
 ghost
 fn gpu_pts_to_ref
   (#a:Type u#0)
-  (#sz:nat)
   (#f : perm)
-  (x:gpu_array a sz)
+  (x : array a)
   (#v : seq a)
-  preserves x |-> Frac f v
-  ensures  pure (Seq.length v == sz /\ SZ.fits sz)
+  preserves
+    x |-> Frac f v
+  ensures
+    pure (Seq.length v == Pulse.Lib.Array.length x /\ SZ.fits (Pulse.Lib.Array.length x))
 {
-  gpu_pts_to_slice_ref x 0 sz;
+  Pulse.Lib.Array.pts_to_len x;
+  ();
 }
 
 
 ghost
 fn gpu_pts_to_ref_located
   (#a:Type u#0)
-  (#sz:nat)
   (#f : perm)
-  (x:gpu_array a sz)
+  (x : array a)
   (#v : seq a)
   (#l : loc_id)
-  preserves on l (x |-> Frac f v)
-  ensures  pure (Seq.length v == sz /\ SZ.fits sz)
+  preserves
+    on l (x |-> Frac f v)
+  ensures
+    pure (Seq.length v == Pulse.Lib.Array.length x /\ SZ.fits (Pulse.Lib.Array.length x))
 {
   ghost_impersonate l
     (on l (x |-> Frac f v))
-    (on l (x |-> Frac f v) ** pure (Seq.length v == sz /\ SZ.fits sz))
+    (on l (x |-> Frac f v) ** pure (Seq.length v == Pulse.Lib.Array.length x /\ SZ.fits (Pulse.Lib.Array.length x)))
     fn () {
       on_elim _;
       gpu_pts_to_ref x;
@@ -57,32 +60,32 @@ ghost
 fn gpu_slice_split'
   (#a:Type u#0)
   (#sz:nat)
-  (arr : gpu_array a sz)
+  (arr : larray a sz)
   (#[exact (`1.0R)] f : perm)
   (#s : erased (seq a))
   (i n : nat)
   (#_ : squash (0 <= n-i /\ n-i < length s))
   (m:nat)
-  requires gpu_pts_to_slice arr #f i m s ** pure (n <= m)
-  ensures  gpu_pts_to_slice arr #f i n (seq_take (n-i) s) ** gpu_pts_to_slice arr #f n m (seq_drop (n-i) s)
+  requires pts_to_slice arr #f i m s ** pure (n <= m)
+  ensures  pts_to_slice arr #f i n (seq_take (n-i) s) ** pts_to_slice arr #f n m (seq_drop (n-i) s)
 {
   assert pure (Seq.equal s (seq_take (n - i) s @+ seq_drop (n - i) s));
-  rewrite gpu_pts_to_slice arr #f i m s
-       as gpu_pts_to_slice arr #f i m (seq_take (n - i) s @+ seq_drop (n - i) s);
-  gpu_slice_split arr #f i n m;
+  rewrite pts_to_slice arr #f i m s
+       as pts_to_slice arr #f i m (seq_take (n - i) s @+ seq_drop (n - i) s);
+  slice_split arr #f i n m;
 }
 
 ghost
 fn gpu_array_unslice_1'
   (#a:Type u#0)
   (#sz:nat)
-  (arr : gpu_array a sz)
+  (arr : larray a sz)
   (#f : perm)
-  requires forall+ (i: natlt sz). exists* v. gpu_pts_to_cell arr #f i v
+  requires forall+ (i: natlt sz). exists* v. pts_to_cell arr #f i v
   ensures  exists* v. pts_to arr #f v
 {
-  let ff = forevery_exists #(natlt sz) (fun i v -> gpu_pts_to_cell arr #f i v);
+  let ff = forevery_exists #(natlt sz) (fun i v -> pts_to_cell arr #f i v);
   let ss = Seq.init_ghost sz (fun i -> ff i);
-  forevery_ext #(natlt sz) _ (fun i -> gpu_pts_to_cell arr #f i (ss @! i));
-  gpu_array_unslice_1 arr;
+  forevery_ext #(natlt sz) _ (fun i -> pts_to_cell arr #f i (ss @! i));
+  array_unslice_1 arr;
 }
