src/lib/data/Kuiper.Array.Vectorized.fsti
@@ -33,88 +33,32 @@ instance has_vec_cpy_half  : has_vec_cpy half =
   Kuiper.Float16.lem_sizeof ();
   { _chunk = 8sz; _pf = ez; }
 
-(* These three operations are essentially the same. We need different
-   variants since gpu_array is a different type from array. Sadly the
-   slicing is also different. The "host" variants are a bit of a
-   misnomer, they are meant to be used with registers arrays, and
-   not CPU-side memory arrays. *)
+(* The single primitive for vectorized copies. *)
 
 noextract (* prevents krml warning *)
-fn gpu_array_vec_cpy_dd
-  (#et : Type u#0) {| sized et, has_vec_cpy et |}
-  (#dst_sz : erased nat)
-  (dst_arr : gpu_array et dst_sz)
-  (dst_off : SZ.t)
-  (#dst_slice_i : erased nat)
-  (#dst_slice_j : erased nat)
-  (#src_sz : erased nat)
-  (#src_slice_i : erased nat)
-  (#src_slice_j : erased nat)
-  (src_arr : gpu_array et src_sz)
-  (src_off : SZ.t)
-  (#f : perm)
-  (#ss : erased (seq et))
-  (#ds : erased (seq et))
-  (#_ : squash (dst_slice_i <= dst_off /\ dst_off + chunk et <= dst_slice_j))
-  (#_ : squash (Seq.length ds == dst_slice_j - dst_slice_i))
-  (#_ : squash (src_slice_i <= src_off /\ src_off + chunk et <= src_slice_j))
-  (#_ : squash (Seq.length ss == src_slice_j - src_slice_i))
-  preserves gpu
-  preserves gpu_pts_to_slice src_arr #f src_slice_i src_slice_j ss
-  requires  pure (aligned' 16 src_arr src_off)
-  requires  pure (aligned' 16 dst_arr dst_off)
-  requires  gpu_pts_to_slice dst_arr dst_slice_i dst_slice_j ds
-  ensures
-    exists* s'.
-      gpu_pts_to_slice dst_arr dst_slice_i dst_slice_j s' **
-      pure (s' == seq_blit ds (dst_off - dst_slice_i) ss (src_off - src_slice_i) (chunk et))
-
-noextract (* prevents krml warning *)
-fn gpu_array_vec_cpy_dh
+fn array_vec_cpy
   (#et : Type u#0) {| sized et, has_vec_cpy et |}
   (dst_arr : array et)
-  (dst_off : SZ.t)
-  (#src_sz : erased nat)
-  (src_arr : gpu_array et src_sz)
-  (src_off : SZ.t)
-  (#src_slice_i : erased nat)
-  (#src_slice_j : erased nat)
-  (#f : perm)
-  (#ss : erased (seq et))
-  (#ds : erased (seq et))
-  (#_ : squash (dst_off + chunk et <= Seq.length ds))
-  (#_ : squash (src_slice_i <= src_off /\ src_off + chunk et <= src_slice_j))
-  (#_ : squash (Seq.length ss == src_slice_j - src_slice_i))
-  preserves gpu
-  preserves gpu_pts_to_slice src_arr #f src_slice_i src_slice_j ss
-  requires  pure (aligned' 16 src_arr src_off)
-  requires  dst_arr |-> ds
-  ensures
-    exists* s'.
-      dst_arr |-> s' **
-      pure (s' == seq_blit ds dst_off ss (src_off - src_slice_i) (chunk et))
-
-noextract (* prevents krml warning *)
-fn gpu_array_vec_cpy_hd
-  (#et : Type u#0) {| sized et, has_vec_cpy et |}
-  (#dst_sz : erased nat)
-  (dst_arr : gpu_array et dst_sz)
   (dst_off : SZ.t)
   (#dst_slice_i : erased nat)
   (#dst_slice_j : erased nat)
   (src_arr : array et)
   (src_off : SZ.t)
+  (#src_slice_i : erased nat)
+  (#src_slice_j : erased nat)
   (#f : perm)
   (#ss : erased (seq et))
   (#ds : erased (seq et))
   (#_ : squash (dst_slice_i <= dst_off /\ dst_off + chunk et <= dst_slice_j))
   (#_ : squash (Seq.length ds == dst_slice_j - dst_slice_i))
-  (#_ : squash (src_off + chunk et <= Seq.length ss))
+  (#_ : squash (src_slice_i <= src_off /\ src_off + chunk et <= src_slice_j))
+  (#_ : squash (Seq.length ss == src_slice_j - src_slice_i))
   preserves gpu
-  preserves src_arr |-> Frac f ss
+  preserves pts_to_slice src_arr #f src_slice_i src_slice_j ss
+  requires  pure (aligned' 16 src_arr src_off)
   requires  pure (aligned' 16 dst_arr dst_off)
-  requires  gpu_pts_to_slice dst_arr dst_slice_i dst_slice_j ds
+  requires  pts_to_slice dst_arr dst_slice_i dst_slice_j ds
   ensures
     exists* s'.
-      gpu_pts_to_slice dst_arr dst_slice_i dst_slice_j s' **
-      pure (s' == seq_blit ds (dst_off - dst_slice_i) ss src_off (chunk et))
+      pts_to_slice dst_arr dst_slice_i dst_slice_j s' **
+      pure (s' == seq_blit ds (dst_off - dst_slice_i) ss (src_off - src_slice_i) (chunk et))
