src/lib/data/Kuiper.Matrix.fst
@@ -33,7 +33,7 @@ let lem_from_array_core
   (#et : Type)
   (#rows #cols : erased nat)
   (#l : mlayout rows cols)
-  (p : gpu_array et (mlayout_size l))
+  (p : larray et (mlayout_size l))
   : Lemma (ensures core (from_array l p) == p)
           [SMTPat (from_array l p)]
   = ()
@@ -131,7 +131,7 @@ fn gpu_matrix_abs
   (#et:Type)
   (#rows #cols : nat)
   (l : mlayout rows cols { is_full_layout l })
-  (p : gpu_array et (mlayout_size l))
+  (p : larray et (mlayout_size l))
   (#f : perm)
   (#em : ematrix et rows cols)
   requires
@@ -156,7 +156,7 @@ fn gpu_matrix_abs'
   (#et:Type)
   (#rows #cols : nat)
   (l : mlayout rows cols { is_full_layout l })
-  (p : gpu_array et (mlayout_size l))
+  (p : larray et (mlayout_size l))
   (#f : perm)
   (#s : lseq et (mlayout_size l))
   requires
@@ -182,7 +182,7 @@ fn gpu_matrix_iconcr
   ensures
     pure (SZ.fits (mlayout_size l)) **
     (forall+ (r : natlt rows) (c : natlt cols).
-      gpu_pts_to_cell (core g) #f (cell_of_pos l r c) (macc em r c))
+      pts_to_cell (core g) #f (cell_of_pos l r c) (macc em r c))
 {
   unfold gpu_matrix_pts_to g #f em;
   A.varray_pts_to_ref g;
@@ -191,7 +191,7 @@ fn gpu_matrix_iconcr
   forevery_rw_type _ (natlt rows & natlt cols) _;
   forevery_unflatten' _;
   forevery_ext_2 _
-    (fun r c -> gpu_pts_to_cell (core g) #f (cell_of_pos l r c) (macc em r c));
+    (fun r c -> pts_to_cell (core g) #f (cell_of_pos l r c) (macc em r c));
 }
 
 ghost
@@ -205,14 +205,14 @@ fn gpu_matrix_iabs
   requires
     pure (SZ.fits (mlayout_size l)) **
     (forall+ (r : natlt rows) (c : natlt cols).
-      gpu_pts_to_cell (core g) #f (cell_of_pos l r c) (macc em r c))
+      pts_to_cell (core g) #f (cell_of_pos l r c) (macc em r c))
   ensures
     g |-> Frac f em
 {
   forevery_flatten _;
   forevery_rw_type _ ((aview_from_mlayout et l).iview.ait) _;
   forevery_ext _
-    (fun i -> gpu_pts_to_cell (A.core g) #f ((aview_from_mlayout et l).iview.step.imap.f i)
+    (fun i -> pts_to_cell (A.core g) #f ((aview_from_mlayout et l).iview.step.imap.f i)
       ((aview_from_mlayout et l).ctn.acc em i));
 
   A.varray_iabs g;
@@ -467,7 +467,7 @@ let gpu_matrix_pts_to_cell_eq
   (v : et)
   : Lemma (gpu_matrix_pts_to_cell gm #f i j v
            ==
-           gpu_pts_to_cell (core gm) #f (cell_of_pos l i j) v)
+           pts_to_cell (core gm) #f (cell_of_pos l i j) v)
   = A.varray_pts_to_cell_eq gm (i,j) f v
 
 inline_for_extraction noextract
