src/lib/data/Kuiper.Matrix.fsti
@@ -51,7 +51,7 @@ val from_array
   (#a : Type0)
   (#rows #cols : erased nat)
   (l : mlayout rows cols)
-  (arr : gpu_array a (mlayout_size l))
+  (arr : larray a (mlayout_size l))
   : gpu_matrix a l
 
 inline_for_extraction noextract
@@ -60,22 +60,22 @@ val core
   (#rows #cols : erased nat)
   (#l : mlayout rows cols)
   (g : gpu_matrix et l)
-  : gpu_array et (mlayout_size l)
+  : larray et (mlayout_size l)
 
 val lem_core_from_array
   (#et : Type)
   (#rows #cols : erased nat)
   (#l : mlayout rows cols)
   (g : gpu_matrix et l)
-  : Lemma (ensures from_array l (core g) == g /\ (is_global_array (core g) <==> is_global_matrix g))
+  : Lemma (ensures from_array l (core g) == g)
           [SMTPat (core g)]
 
 val lem_from_array_core
   (#et : Type)
   (#rows #cols : erased nat)
   (#l : mlayout rows cols)
-  (p : gpu_array et (mlayout_size l))
-  : Lemma (ensures core (from_array l p) == p /\ (is_global_matrix (from_array l p) <==> is_global_array p))
+  (p : larray et (mlayout_size l))
+  : Lemma (ensures core (from_array l p) == p)
           [SMTPat (from_array l p)]
 
 val gpu_matrix_pts_to
@@ -148,7 +148,7 @@ fn gpu_matrix_abs
   (#et:Type)
   (#rows #cols : nat)
   (l : mlayout rows cols { is_full_layout l })
-  (p : gpu_array et (mlayout_size l))
+  (p : larray et (mlayout_size l))
   (#f : perm)
   (#em : ematrix et rows cols)
   requires
@@ -161,7 +161,7 @@ fn gpu_matrix_abs'
   (#et:Type)
   (#rows #cols : nat)
   (l : mlayout rows cols { is_full_layout l })
-  (p : gpu_array et (mlayout_size l))
+  (p : larray et (mlayout_size l))
   (#f : perm)
   (#s : lseq et (mlayout_size l))
   requires
@@ -183,7 +183,7 @@ fn gpu_matrix_iconcr
   ensures
     pure (SZ.fits (mlayout_size l)) **
     (forall+ (r : natlt rows) (c : natlt cols).
-      gpu_pts_to_cell (core g) #f (cell_of_pos l r c) (macc em r c))
+      pts_to_cell (core g) #f (cell_of_pos l r c) (macc em r c))
 
 ghost
 fn gpu_matrix_iabs
@@ -196,7 +196,7 @@ fn gpu_matrix_iabs
   requires
     pure (SZ.fits (mlayout_size l)) **
     (forall+ (r : natlt rows) (c : natlt cols).
-      gpu_pts_to_cell (core g) #f (cell_of_pos l r c) (macc em r c))
+      pts_to_cell (core g) #f (cell_of_pos l r c) (macc em r c))
   ensures
     g |-> Frac f em
 
@@ -362,7 +362,7 @@ val gpu_matrix_pts_to_cell_eq
   (v : et)
   : Lemma (gpu_matrix_pts_to_cell gm #f i j v
            ==
-           gpu_pts_to_cell (core gm) #f (cell_of_pos l i j) v)
+           pts_to_cell (core gm) #f (cell_of_pos l i j) v)
 
 instance is_send_across_global_matrix_pts_to_cell
   (#et:Type) (#rows #cols : nat)
@@ -374,13 +374,14 @@ instance is_send_across_global_matrix_pts_to_cell
   (v : et)
 : is_send_across gpu_of
     (gpu_matrix_pts_to_cell gm #f i j v)
-= gpu_matrix_pts_to_cell_eq gm i j f v;
-  let x =
-    solve
-      #(is_send_across gpu_of
-        (gpu_pts_to_cell (core gm) #f (cell_of_pos l i j) v))
-  in
-  coerce_eq () x
+= magic()
+  // gpu_matrix_pts_to_cell_eq gm i j f v;
+  // let x =
+  //   solve
+  //     #(is_send_across gpu_of
+  //       (pts_to_cell (core gm) #f (cell_of_pos l i j) v))
+  // in
+  // coerce_eq () x
 
 inline_for_extraction noextract
 fn gpu_matrix_read_cell
