src/lib/data/Kuiper.Tensor.fsti
@@ -23,7 +23,7 @@ inline_for_extraction noextract
 val from_array
   (#et : Type0) (#r : erased nat) (#d : idesc r)
   (l : tlayout d)
-  (a : gpu_array et (tlayout_size l))
+  (a : larray et (tlayout_size l))
   : tensor et l
 
 inline_for_extraction noextract
@@ -31,7 +31,7 @@ val core
   (#et : Type0) (#r : erased nat) (#d : idesc r)
   (#l : tlayout d)
   (a : tensor et l)
-  : gpu_array et (tlayout_size l)
+  : larray et (tlayout_size l)
 
 val lem_core_from_array
   (#et : Type0) (#r : nat) (#d : idesc r)
@@ -43,7 +43,7 @@ val lem_core_from_array
 val lem_from_array_core
   (#et : Type0) (#r : nat) (#d : idesc r)
   (#l : tlayout d)
-  (p : gpu_array et (tlayout_size l))
+  (p : larray et (tlayout_size l))
   : Lemma (ensures core (from_array l p) == p)
           [SMTPat (from_array l p)]
 
@@ -151,7 +151,7 @@ fn tensor_abs
   (#et:Type)
   (#r : nat) (#d : idesc r)
   (l : tlayout d { is_full l })
-  (p : gpu_array et (tlayout_size l))
+  (p : larray et (tlayout_size l))
   (#f : perm)
   (#s : chest d et)
   requires
@@ -164,7 +164,7 @@ fn tensor_abs'
   (#et:Type)
   (#r : nat) (#d : idesc r)
   (l : tlayout d { is_full l })
-  (p : gpu_array et (tlayout_size l))
+  (p : larray et (tlayout_size l))
   (#f : perm)
   (#s : lseq et (tlayout_size l))
   requires
@@ -283,7 +283,7 @@ val tensor_pts_to_cell_eq
   (a : tensor et l) (i : abs d) (f : perm) (v : et)
   : Lemma (Cell a i |-> Frac f v
            ==
-           gpu_pts_to_cell (core a) #f (l.imap.f i) v)
+           pts_to_cell (core a) #f (l.imap.f i) v)
 
 instance
 val is_send_across_global_tensor_cell
@@ -333,7 +333,7 @@ fn tensor_ilower
   ensures
     pure (SZ.fits (tlayout_size l)) **
     (forall+ (i : abs d).
-      gpu_pts_to_cell (core a) #f (l.imap.f i) (acc s i))
+      pts_to_cell (core a) #f (l.imap.f i) (acc s i))
 
 ghost
 fn tensor_iraise
@@ -345,7 +345,7 @@ fn tensor_iraise
   requires
     pure (SZ.fits (tlayout_size l)) **
     (forall+ (i : abs d).
-      gpu_pts_to_cell (core a) #f (l.imap.f i) (acc s i))
+      pts_to_cell (core a) #f (l.imap.f i) (acc s i))
   ensures
     a |-> Frac f s
 
