src/lib/ghost/Kuiper.Ghost.TensorTranspose.fst
@@ -47,6 +47,7 @@ fn ghost_transpose1
 }
 #pop-options
 
+#push-options "--z3rlimit 40 --retry 3"
 ghost
 fn ghost_transpose2
   (#et:Type)
@@ -66,6 +67,7 @@ fn ghost_transpose2
        as core gA |-> to_seq (l2_row_major cols rows) (mtranspose m);
   raise (l2_row_major cols rows) (core gA);
 }
+#pop-options
 
 ghost
 fn ghost_transpose1_back
